Commit

Compiler/CompilerProof.v
@@ -1,5 +1,18 @@
-Require Import TypedTerm Monad Host DepList CUDALib Compiler Correctness CodeGenM.
+Require Import LibTactics assertion_lemmas GPUCSL TypedTerm Monad
+        Host DepList CUDALib CSLLemma CSLTactics Compiler Correctness CodeGenM.
 
-Theorem compile_prog_ok GA ty ntrd nblk (p : Skel.AS GA ty) :
+
+Definition main_spec GA :=
+  let ps := gen_params GA in
+  let params := flatten_avars (hmap (fun ty x => ((fst (fst x), Int), toPtr (snd x))) ps) in
+  {| fs_tag := Hfun; fs_params := map fst params;
+     fs_tri := (All (apEnv : APtrEnv GA) (aeEnv : AEvalEnv GA),
+                FDbl (kernelInv (remove_typeinfo ps) apEnv aeEnv Emp True nil 1)
+                     ((fun _ _ => True) ** (kernelInv (remove_typeinfo ps) apEnv aeEnv Emp True nil 1))) |}.
+
+Theorem compile_AS_ok GA ty ntrd nblk (p : Skel.AS GA ty) :
   let M := compile_prog ntrd nblk p in
-  sat_FC M nil ("__main", {|fs_tag := Hfun; fs_params := |})
+  sat_FC M nil (("__main", main_spec GA) :: nil).
+Proof.
+  admit.
+Qed.
